proof-libs/fstar/core/Core.Ops.Arith.fsti
@@ -2,7 +2,7 @@ module Core.Ops.Arith
 open Rust_primitives
 
 
-class t_Add self rhs = {
+class t_Add #self #rhs = {
    [@@@ Tactics.Typeclasses.no_method]
    f_Output: Type;
    f_add_pre: self -> rhs -> bool;
@@ -10,7 +10,7 @@ class t_Add self rhs = {
    f_add: x:self -> y:rhs -> Pure f_Output (f_add_pre x y) (fun r -> f_add_post x y r);
 }
 
-class t_Sub self rhs = {
+class t_Sub #self #rhs = {
    [@@@ Tactics.Typeclasses.no_method]
    f_Output: Type;
    f_sub_pre: self -> rhs -> bool;
@@ -18,7 +18,7 @@ class t_Sub self rhs = {
    f_sub: x:self -> y:rhs -> Pure f_Output (f_sub_pre x y) (fun r -> f_sub_post x y r);
 }
 
-class t_Mul self rhs = {
+class t_Mul #self #rhs = {
    [@@@ Tactics.Typeclasses.no_method]
    f_Output: Type;
    f_mul_pre: self -> rhs -> bool;
@@ -26,7 +26,7 @@ class t_Mul self rhs = {
    f_mul: x:self -> y:rhs -> Pure f_Output (f_mul_pre x y) (fun r -> f_mul_post x y r);
 }
 
-class t_Div self rhs = {
+class t_Div #self #rhs = {
    [@@@ Tactics.Typeclasses.no_method]
    f_Output: Type;
    f_div_pre: self -> rhs -> bool;
@@ -34,13 +34,13 @@ class t_Div self rhs = {
    f_div: x:self -> y:rhs -> Pure f_Output (f_div_pre x y) (fun r -> f_div_post x y r);
 }
 
-class t_AddAssign self rhs = {
+class t_AddAssign #self #rhs = {
   f_add_assign_pre: self -> rhs -> bool;
   f_add_assign_post: self -> rhs -> self -> bool;
   f_add_assign: x:self -> y:rhs -> Pure self (f_add_assign_pre x y) (fun r -> f_add_assign_post x y r);
 }
 
-class t_SubAssign self rhs = {
+class t_SubAssign #self #rhs = {
   f_sub_assign_pre: self -> rhs -> bool;
   f_sub_assign_post: self -> rhs -> self -> bool;
   f_sub_assign: x:self -> y:rhs -> Pure self (f_sub_assign_pre x y) (fun r -> f_sub_assign_post x y r);
