proof-libs/fstar/rust_primitives/Rust_primitives.Hax.fst
@@ -10,9 +10,9 @@ let repeat #a (x: a) (len: usize): t_Array a len =
   FStar.Seq.create (v len) x
 
 open Core.Ops.Index
-class update_at_tc self idx = {
+class update_at_tc #self #idx = {
   [@@@FStar.Tactics.Typeclasses.tcinstance]
-  super_index: t_Index self idx;
+  super_index: t_Index #self #idx;
   update_at: s: self -> i: idx {f_index_pre s i} -> super_index.f_Output -> self;
 }
 
@@ -21,7 +21,7 @@ open Core.Slice
 /// We have an instance for `int_t n`, but we often work with refined
 /// `int_t n`, and F* typeclass inference doesn't support subtyping
 /// well, hence the instance below.
-instance impl__index_refined t l n r: t_Index (t_Array t l) (x: int_t n {r x})
+instance impl__index_refined t l n r: t_Index #(t_Array t l) #(x: int_t n {r x})
   = { f_Output = t;
       f_index_pre = (fun (s: t_Array t l) (i: int_t n {r i}) -> v i >= 0 && v i < v l);
       f_index_post = (fun _ _ _ -> true);
@@ -30,24 +30,24 @@ instance impl__index_refined t l n r: t_Index (t_Array t l) (x: int_t n {r x})
 
 /// Similarly to `impl__index_refined`, we need to define a instance
 /// for refined `int_t n`.
-instance update_at_tc_array_refined t l n r: update_at_tc (t_Array t l) (x: int_t n {r x}) = {
+instance update_at_tc_array_refined t l n r: update_at_tc #(t_Array t l) #(x: int_t n {r x}) = {
   super_index = impl__index_refined t l n r;
   update_at = (fun arr i x -> FStar.Seq.upd arr (v i) x);
 }
 
-instance impl__index t l n: t_Index (t_Array t l) (int_t n)
+instance impl__index t l n: t_Index #(t_Array t l) #(int_t n)
   = { f_Output = t;
       f_index_pre = (fun (s: t_Array t l) (i: int_t n) -> v i >= 0 && v i < v l);
       f_index_post = (fun _ _ _ -> true);
       f_index = (fun s i -> Seq.index s (v i));
     }
 
-instance update_at_tc_array t l n: update_at_tc (t_Array t l) (int_t n) = {
-  super_index = FStar.Tactics.Typeclasses.solve <: t_Index (t_Array t l) (int_t n);
+instance update_at_tc_array t l n: update_at_tc #(t_Array t l) #(int_t n) = {
+  super_index = FStar.Tactics.Typeclasses.solve <: t_Index #(t_Array t l) #(int_t n);
   update_at = (fun arr i x -> FStar.Seq.upd arr (v i) x);
 }
 
-let (.[]<-) #self #idx {| update_at_tc self idx |} (s: self) (i: idx {f_index_pre s i})
+let (.[]<-) #self #idx {| update_at_tc #self #idx |} (s: self) (i: idx {f_index_pre s i})
   = update_at s i
 
 let array_of_list (#t:Type)
