proof-libs/fstar/core/Core.Clone.fst
@@ -1,11 +1,11 @@
 module Core.Clone
 
-class t_Clone self = {
+class t_Clone #self = {
   f_clone: x:self -> r:self {x == r}
 }
 
 (** Everything is clonable *)
-instance clone_all (t: Type): t_Clone t = {
+instance clone_all (t: Type): t_Clone #t = {
   f_clone = (fun x -> x);
 }
 
