proof-libs/fstar/core/Core.Ops.Try_trait.fst
@@ -1,14 +1,14 @@
 module Core.Ops.Try_trait
 
-class t_FromResidual self r = {
+class t_FromResidual #self #r = {
    f_from_residual: r -> self;
 }
 
-class t_Try self = {
+class t_Try #self = {
    f_Output: Type0;
    f_Residual: Type0;
    [@@@FStar.Tactics.Typeclasses.tcresolve]
-   parent_FromResidual: t_FromResidual f_Residual f_Residual;
+   parent_FromResidual: t_FromResidual #f_Residual #f_Residual;
 
    f_from_output: f_Output -> self;
    f_branch: self -> Core.Ops.Control_flow.t_ControlFlow f_Residual f_Output;
